@prefix ro: <https://w3id.org/ro/crate/1.0/context#> .
@prefix da: <https://open-vocabularies.vliz.be/dmbonassistant#> .
@prefix owl: <http://www.w3.org/2002/07/owl#> .
@prefix dc: <http://purl.org/dc/terms/> .
@prefix schema: <http://schema.org/> .
@prefix foaf: <http://xmlns.com/foaf/0.1/> .
@prefix rdf: <http://www.w3.org/1999/02/22-rdf-syntax-ns#> .
@prefix rdfs: <http://www.w3.org/2000/01/rdf-schema#> .
@prefix xsd: <http://www.w3.org/2001/XMLSchema#> .
@prefix skos: <http://www.w3.org/2004/02/skos/core#> .
@prefix vann:   <http://purl.org/vocab/vann/> .


<https://open-vocabularies.vliz.be/dmbonassistant>
    a owl:Ontology;
    rdfs:label       "dmbon-assistant-ontology"@en ;
    rdfs:comment     "The DMBON Assistant ontology"@en ;
    dc:issued        "2022-05-06"^^xsd:date ;
    dc:modified      "2022-06-22"^^xsd:date ;
    dc:license       <https://creativecommons.org/licenses/by/4.0/> ;
    dc:creator
    [
        schema:name         "VLIZ Open Science team" ;
        schema:email        <mailto:opsci@vliz.org> ;
	      schema:affiliation  <https://www.vliz.be/> ;
    ] ;
    dc:contributor
    [
        schema:name         "Laurian Van Maldeghem" ;
        schema:identifier   <https://orcid.org/0000-0003-0663-5907> ;
        schema:email        <mailto:laurian.van.maldeghem@vliz.be> ;
        schema:affiliation  <https://www.vliz.be/> ;
    ],
    [
        schema:name         "Marc Portier" ;
        schema:identifier   <https://orcid.org/0000-0002-9648-6484> ;
        schema:email        <mailto:marc.portier@vliz.be> ;
        schema:affiliation  <https://www.vliz.be/> ;
    ],
    [
        schema:name         "Cedric Decruw" ;
        schema:identifier   <https://orcid.org/0000-0001-6387-5988> ;
        schema:email        <mailto:cedric.decruw@vliz.be> ;
        schema:affiliation  <https://www.vliz.be/> ;
    ] ;
    vann:preferredNamespacePrefix "da" ;
    vann:preferredNamespaceUri    "https://open-vocabularies.vliz.be/dmbonassistant#" .


<https://www.vliz.be/>
  a schema:Organization ;
  schema:name   "Vlaams Instituut voor de Zee"@nl ;
  schema:name   "Flanders Marine Institute"@en ;
  schema:url    <https://www.vliz.be/> .


### classes ###

da:SeedCrate
  a                     skos:Concept ;
  rdfs:isDefinedBy      <https://open-vocabularies.vliz.be/dmbonassistant>;
  rdfs:comment          """A seed-RO-Crate is a kind of template/empty data-package containing structure and files to be filled in.
  The cloning of the seed-crate marks the beginning of the management of a specific data-RO-Crate."""@en ;
  rdfs:label            "Seed RO-Crate"@en ;
  rdfs:subclassof	      ro:CreativeWork .

da:CrateRepo
  a                     skos:Concept ;
  rdfs:isDefinedBy      <https://open-vocabularies.vliz.be/dmbonassistant>;
  rdfs:comment          "The access-string to the (public) file repository holding the version managed source data files of the RO-Crate datapackage."@en ;
  rdfs:label            "RO-Crate repository"@en ;
  rdfs:subclassof	      ro:RepositoryObject .
# to check with Cedric if this is correct... --> atm points to collection class, while the expected value should be a url??
# in fact - a git-connect-string is technically not a URL - since it does not start with http(s)://

da:SpaceUrl
  a                     skos:Concept ;
  rdfs:isDefinedBy      <https://open-vocabularies.vliz.be/dmbonassistant>;
  rdfs:comment          "The link to the Space of the RO-Crate."@en ;
  rdfs:label            "RO-Crate Space URL"@en ;
  rdfs:subclassof	      ro:URL .

da:ShaclFile
  a                     skos:Concept ;
  rdfs:isDefinedBy      <https://open-vocabularies.vliz.be/dmbonassistant>;
  rdfs:comment          "The SHACL file with the contrains to which the RO-Crate data is/should be conformant."@en ;
  rdfs:label            "RO-Crate SHACL file"@en ;
  rdfs:subclassof	      ro:File .

da:SemUpliftFile
  a                     skos:Concept ;
  rdfs:isDefinedBy      <https://open-vocabularies.vliz.be/dmbonassistant>;
  rdfs:comment          "The PySUByT templates files used to semantically uplift the RO-Crate."@en ;
  rdfs:label            "RO-Crate semantic uplifting file(s)"@en ;
  rdfs:subclassof	      ro:File .


### predicates ###

da:crateRepo
  a 			owl:ObjectProperty ; 
  rdfs:isDefinedBy      <https://open-vocabularies.vliz.be/dmbonassistant>;
  rdfs:comment          "Indicates a RO-Crate repo."@en ;
  rdfs:label            "RO-Crate repo"@en ;
  rdfs:domain           ro:CreativeWork ;
  rdfs:range            da:SeedCrate .

da:semBenchConfigPath
  a 			owl:ObjectProperty ; 
  rdfs:isDefinedBy      <https://open-vocabularies.vliz.be/dmbonassistant>;
  rdfs:comment          "A configuration file for semantic workbench actions"@en ;
  rdfs:label            "sembench config file"@en ;
  rdfs:domain           ro:CreativeWork ;
  rdfs:range            da:SeedCrate .

da:hasSeedCrate
  a                     owl:ObjectProperty ;
  rdfs:isDefinedBy      <https://open-vocabularies.vliz.be/dmbonassistant>;
  rdfs:comment          "Indicates the seed RO-Crate, which is the RO-Crate used as a template to start and manage datapackages conforming to this RO-Profile-Crate."@en ;
  rdfs:label            "Has seed RO-Crate"@en ;
  rdfs:domain           ro:CreativeWork ;
  rdfs:range            da:SeedCrate .


da:hasCrateRepo
  a                     owl:ObjectProperty ;
  rdfs:isDefinedBy      <https://open-vocabularies.vliz.be/dmbonassistant>;
  rdfs:comment          "Indicates the GitHub repository of the RO-Crate."@en ;
  rdfs:label            "Has RO-Crate repository"@en ;
  rdfs:domain           ro:CreativeWork ;
  rdfs:range            da:CrateRepo .


da:hasSpace
  a                     owl:ObjectProperty ;
  rdfs:isDefinedBy      <https://open-vocabularies.vliz.be/dmbonassistant>;
  rdfs:comment          "Indicates the DM BON assistant 'Space' of the RO-Crate."@en ;
  rdfs:label            "Has Space"@en ;
  rdfs:domain           ro:CreativeWork ;
  rdfs:range            da:SpaceUrl .


da:hasShaclFile
  a                     owl:ObjectProperty ;
  rdfs:isDefinedBy      <https://open-vocabularies.vliz.be/dmbonassistant>;
  rdfs:comment          "Indicates the shacl constrains that are applied to the RO-Crate."@en ;
  rdfs:label            "Has Shacl constrains"@en ;
  rdfs:domain           ro:CreativeWork ;
  rdfs:range            da:ShaclFile .


da:hasSemUpliftFile
  a                     owl:ObjectProperty ;
  rdfs:isDefinedBy      <https://open-vocabularies.vliz.be/dmbonassistant>;
  rdfs:comment          "Indicates the PySUByT template(s) used to semantically uplift the data within the RO-Crate."@en ;
  rdfs:label            "Has uplifting templates"@en ;
  rdfs:domain           ro:CreativeWork ;
  rdfs:range            da:SemUpliftFile .